% !TEX root = ../MA119-Question-Bank.tex



\pgfmathtruncatemacro{\a}{random(1,3)} 

\pgfmathtruncatemacro{\b}{random(2,4)}


\pgfmathtruncatemacro{\c}{random(1,5)}




\pgfmathtruncatemacro{\minit}{random(1,3)-2} 
\pgfmathtruncatemacro{\m}{ifthenelse(\minit<0,\minit,\minit+1)} 
\pgfmathtruncatemacro{\oppm}{-\m} 


\pgfmathtruncatemacro{\n}{random(2,3)} 

\pgfmathtruncatemacro{\ansonea}{-\a*\m^2+\b*\m-\c} 
\pgfmathtruncatemacro{\ansoneb}{-\a*(\oppm)^2+\b*(\oppm)-\c} 
\pgfmathtruncatemacro{\ansone}{\ansonea+\ansoneb} 


\pgfmathtruncatemacro{\at}{\a*(\n)^2}
\pgfmathtruncatemacro{\bt}{\b*\n} 



 



If $f(x)=-\ifnum \a=1 \else \a\fi   x^2  + \ifnum\b=1 \else \b\fi  x  -  \c$, 
determine the function values 

\begin{enumerate*}[label={\textup(\arabic*)}, afterlabel=~~~, itemjoin=\hspace{0.25\textwidth}]
\item $f(\m)+f(\oppm)$, 
\item $f(\n t)$.
\end{enumerate*}


\begin{solution}
\begin{enumerate}[label={\textup(\arabic*)}, afterlabel=~~~]
\item
Since
\[
f(\m)=-\ifnum\a=1  \else \a \fi (\m)^2    + \ifnum\b=1 \else \b  \fi  (\m)  -  \c=\ansonea,
\]
and
\[
f(\oppm)=-\ifnum\a=1  \else \a \fi (\oppm)^2    + \ifnum\b=1 \else \b  \fi  (\oppm)  -  \c=\ansoneb.
\]
Then
\[f(\m)+f(\oppm)=\ansonea+ \display{\ansoneb}=\ansone.\]

\item 
\[
f(\n t)
=-\ifnum\a=1 \else \a \fi (\n t)^2+ \ifnum\b=1 \else \b\fi  (\n t)-\c
= -\ifnum\at=1 \else \at \fi t^2  \ifnum\bt=1 + \else \ifnum\bt=-1  - \else +\bt \fi \fi  t-\c
\]
\end{enumerate}
\end{solution}