% !TEX root = ../MA119-Question-Bank.tex




% \pgfmathtruncatemacro{\a}{random(1,5)}
% \pgfmathtruncatemacro{\k}{\a^2}

% \pgfmathdeclarerandomlist{diffone}{{2}{3}{4}{5}}
% \pgfmathdeclarerandomlist{difftwo}{{1}{3}{4}{5}}
% \pgfmathdeclarerandomlist{diffthree}{{1}{2}{4}{5}}
% \pgfmathdeclarerandomlist{difffour}{{1}{2}{3}{5}}
% \pgfmathdeclarerandomlist{difffive}{{1}{2}{3}{4}}

% \ifcase\a\relax%
%   \or \pgfmathrandomitem{\h}{diffone}
%   \or \pgfmathrandomitem{\h}{difftwo}
%   \or \pgfmathrandomitem{\h}{diffthree}
%   \or \pgfmathrandomitem{\h}{difffour}
%   \or \pgfmathrandomitem{\h}{difffive} 
%  \fi
%  \edef\h{\h}

\pgfmathtruncatemacro{\c}{random(1,2)}
\pgfmathtruncatemacro{\coef}{random(2,11)}
\pgfmathtruncatemacro{\tentopowerc}{10^\c}
\pgfmathtruncatemacro{\a}{\tentopowerc-\coef}
\pgfmathtruncatemacro{\ans}{-random(2, 5)}
\pgfmathtruncatemacro{\negans}{-\ans}
\pgfmathtruncatemacro{\b}{-\coef*\ans}

Solve the logarithmic equation 
\[\log(\b-\a x)=\c+\log(-x).\]


\begin{solution}
		\[\begin{split}
		\log(\b-\a x)&=\c+\log(-x)\\
		\log(\b-\a x)-\log(-x)&=\c\\
		\log\left(\frac{\b-\a x}{-x}\right)&=\c\\
		 \frac{\b-\a x}{-x} &=10^\c\\
		  \frac{\b-\a x}{-x} &=\tentopowerc\\
		  \b-\a x&=-\tentopowerc x\\
		  \b&=-\coef x\\
		  x&=\ans.
		\end{split}
		\]
Check: The left hand side is 
\[\log(\b-\a\cdot (\ans))=\log(\negans\cdot\tentopowerc)=\log\negans+\c\]
which is the same as right hand side.
So the solution is $x=\ans$.
\end{solution}
