% !TEX root = ../MA119-Question-Bank.tex


%%%%%%The solution (x, y)
\pgfmathtruncatemacro{\x}{random(1,3)-2} 
\pgfmathtruncatemacro{\y}{-random(1,4)+3}


%%%%Coeff of equation 1
\pgfmathtruncatemacro{\aone}{-random(1,3)} %%coef of x
\pgfmathtruncatemacro{\bone}{random(1,3)}


%%%%Coeff of equation 2
\pgfmathtruncatemacro{\atwo}{2} %%coef of x
\pgfmathtruncatemacro{\btwo}{1}


%%%%least common multiple of coeff of y
\pgfmathtruncatemacro{\lcmy}{\bone*\btwo/gcd(\bone,\btwo)}


%%%%Multipliers
\pgfmathtruncatemacro{\money}{\lcmy/\bone}
\pgfmathtruncatemacro{\mtwoy}{\lcmy/\btwo}


%%%%% new a's after multiply by the multipliers
\pgfmathtruncatemacro{\maone}{\money*\aone}
\pgfmathtruncatemacro{\matwo}{\mtwoy*\atwo}


%%%%%%original c's
\pgfmathtruncatemacro{\cone}{\aone*\x-\bone*\y}
\pgfmathtruncatemacro{\ctwo}{\atwo*\x-\btwo*\y}


%%%%%%new c's
\pgfmathtruncatemacro{\monecone}{\money*\cone}
\pgfmathtruncatemacro{\mtwoctwo}{\mtwoy*\ctwo}


%%%%%% coeff of x after eliminating y
\pgfmathtruncatemacro{\coefx}{\maone-\matwo}

%%%%%%right side number after eliminating
\pgfmathtruncatemacro{\cthree}{\monecone-\mtwoctwo}


%%%%%% a_1 times \x
\pgfmathtruncatemacro{\aonetimesx}{\aone*\x}


%%%%%% c_1 minus aone\x
\pgfmathtruncatemacro{\coneminusaonex}{\cone-\aone*\x}




\setcounter{equation}{0}


Solve the following system of linear equations.
\begin{align}
\displayaone x - \displaybone y &= \cone  \label{eq-I003-1}\\
\displayatwo x - \displaybtwo y &= \ctwo  \label{eq-I003-2}
\end{align}

\begin{solution}

\ifnum\bone=1 
	Multiply \eqref{eq-I003-1} by $\money$.
		\begin{align}
		\money(\displayaone x) - \money(\displaybone y) &=\money\cdot(\cone) \nonumber \\
		\maone x - \lcmy y &= \monecone \label{eq-I003-3}
		\end{align}

\else 
	\ifnum\btwo=1
		Multiply \eqref{eq-I003-2} by $\mtwoy$.
		\begin{align}
		\mtwoy(\displayatwo x) - \mtwoy(\displaybtwo y) &=\mtwoy\cdot(\ctwo) \nonumber \\
		\matwo x - \lcmy y &= \mtwoctwo \label{eq-I003-4}
		\end{align}
	\else
		Multiply \eqref{eq-I003-1} by $\money$ and \eqref{eq-I003-2} by $\mtwoy$.
		\begin{align}
		\money(\displayaone x) - \money(\displaybone y) &=\money\cdot(\cone) \nonumber \\
		\maone x - \lcmy y &= \monecone \label{eq-I003-3}
		\end{align}

		\begin{align}
		\mtwoy(\displayatwo x) - \mtwoy(\displaybtwo y) &=\mtwoy\cdot(\ctwo) \nonumber \\
		\matwo x - \lcmy y &= \mtwoctwo \label{eq-I003-4}
		\end{align}

	\fi
\fi

Subtraction equations to eliminate $y$: \eqref{eq-I003-1}$-$\eqref{eq-I003-4} 
\begin{align}
&& \maone x - \lcmy y &= \monecone \nonumber \\
-&& \matwo x - \lcmy y &= \mtwoctwo  \nonumber\\[-0.5em]
\cline{1-4}
&& \displaycoefx x+0 &=\cthree \nonumber\\
&& x&=\x\nonumber
\end{align}



Plug $x=\x$ into \eqref{eq-I003-1} and solve for $y$.
\begin{align*}
\aone\cdot \x- \displaybone y &=\cone \\
\aonetimesx-\displaybone y&= \cone\\
-\displaybone y&= \coneminusaonex \\
y&=\y
\end{align*}
% \end{enumerate}
The solution is $(\x,\y)$. 

\end{solution}
